unity/scheduling/basic.lean
@@ -1,48 +1,158 @@
 
 import data.stream
 import unity.temporal
+import unity.logic
 import util.data.bijection
 import util.data.stream
 
+universe variables u
+
 namespace scheduling
-
-variable {lbl : Type}
-
-structure fair {lbl : Type} (req : stream (set lbl)) (τ : stream lbl) : Prop :=
-  (valid : ∀ i, req i = ∅ ∨ τ i ∈ req i)
-  (fair : ∀ l, ([]<>•mem l) req → ([]<>•eq l) τ)
 
 open stream nat
 
-def req_of {lbl} (r : list lbl → set lbl) (τ : stream lbl) : stream (set lbl) :=
+section
+
+parameters {lbl : Type}
+
+structure fair (req : stream (set lbl)) (τ : stream lbl) : Prop :=
+  (valid : ∀ i, req i = ∅ ∨ τ i ∈ req i)
+  (fair : ∀ l, ([]<>•mem l) req → ([]<>•eq l) τ)
+
+def req_of (r : list lbl → set lbl) (τ : stream lbl) : stream (set lbl) :=
 λ i, r (approx i τ)
 
-lemma req_of_comp_length {lbl} (r : stream (set lbl)) (τ : stream lbl)
+lemma req_of_comp_length (r : stream (set lbl)) (τ : stream lbl)
 : req_of (r ∘ list.length) τ = r :=
 begin
   unfold req_of function.comp,
   simp [length_approx],
 end
 
-lemma req_of_succ {lbl} (r : list lbl → set lbl) (τ : stream lbl) (i : ℕ)
+lemma req_of_succ (r : list lbl → set lbl) (τ : stream lbl) (i : ℕ)
 : req_of r τ (succ i) = req_of (r ∘ flip list.concat (τ i)) τ i :=
 begin
   unfold req_of function.comp flip,
   rw approx_succ_eq_concat,
 end
 
-class inductive sched (lbl : Type)
-  | fin : finite lbl → sched
-  | inf : infinite lbl → sched
+class inductive sched (l : Type)
+  | fin : finite l → sched
+  | inf : infinite l → sched
 
-instance fin_sched {lbl : Type} [pos_finite lbl] : sched lbl :=
+instance fin_sched [pos_finite lbl] : sched lbl :=
 sched.fin (by apply_instance)
 
-instance inf_sched {lbl : Type} [infinite lbl] : sched lbl :=
+instance inf_sched [infinite lbl] : sched lbl :=
 sched.inf (by apply_instance)
 
-instance sched_option_inf {lbl : Type} : ∀ [sched lbl], sched (option lbl)
+instance sched_option_inf : ∀ [sched lbl], sched (option lbl)
   | (sched.inf inf) := sched.inf (by apply_instance)
   | (sched.fin fin) := sched.fin (by apply_instance)
+
+end
+
+namespace unity
+
+section
+
+open unity
+
+parameters {lbl : Type}
+parameters {s : Type u}
+parameters [system_sem s]
+parameters r : list lbl → set lbl
+parameters {F : s}
+parameters ch : unity.state s → lbl
+parameters hist : unity.state s → list lbl
+def req (σ) := r (hist σ)
+parameters P : ∀ l, often_imp_often F (mem l ∘ req) (eq l ∘ ch)
+parameters INIT : system.init F (eq [ ] ∘ hist)
+parameters STEP : unity.co' F (λ σ σ', hist σ' = hist σ ++ [ch σ])
+parameters INV : ∀ σ, req σ = ∅ ∨ ch σ ∈ req σ
+
+include INIT STEP
+
+section
+
+lemma keep_history {τ : stream (unity.state s)} (i : ℕ)
+  (h : system_sem.ex F τ)
+: approx i (map ch τ) = hist (τ i) :=
+begin
+  induction i with i IH,
+  { note h' := system_sem.init_sem INIT τ h,
+    unfold temporal.init function.comp at h',
+    rw -h', refl },
+  { rw [stream.approx_succ_eq_append,IH],
+    unfold map nth,
+    symmetry,
+    apply STEP,
+    note h' := system_sem.safety _ _ h i,
+    rw temporal.action_drop at h',
+    apply h' },
+end
+
+end
+
+include F
+
+lemma local_req (τ : stream (unity.state s))
+  (h : system_sem.ex F τ)
+  (i : ℕ)
+: req_of r (map ch τ) i = r (hist $ τ i) :=
+begin
+  unfold req_of,
+  rw keep_history _ _ INIT STEP i h,
+end
+
+include ch P hist INV
+
+lemma scheduling'
+: ∃ τ : stream lbl, fair (req_of r τ) τ :=
+begin
+  apply exists_imp_exists' (stream.map ch) _ (system_sem.inhabited F),
+  intros τ sem,
+  apply fair.mk,
+  { intro i,
+    rw local_req _ _ _ INIT STEP _ sem i,
+    unfold map nth,
+    apply INV, },
+  { intro l,
+    assert h : req_of r (map ch τ) = (function.comp (req r hist) τ),
+    { apply funext (local_req _ _ _ INIT STEP _ sem) },
+    assert h' : (map ch τ) = ch ∘ τ,
+    { refl },
+    rw [h,-temporal.inf_often_trace_init_trading],
+    rw [h',-temporal.inf_often_trace_init_trading _ ch],
+    apply system_sem.often_imp_often_sem' _ sem,
+    apply P }
+end
+
+end
+
+open unity
+
+variable {lbl : Type}
+variable r : list lbl → set lbl
+
+structure scheduler :=
+ (s : Type u)
+ (sem : system_sem s)
+ (F : s)
+ (ch : unity.state s → lbl)
+ (hist : unity.state s → list lbl)
+ (req := λ σ, r (hist σ))
+ (INIT : system.init F (eq [ ] ∘ hist))
+ (STEP : unity.co' F (λ σ σ', hist σ' = hist σ ++ [ch σ]))
+ (INV  : ∀ σ, req σ = ∅ ∨ ch σ ∈ req σ)
+ (PROG : ∀ l, often_imp_often F (mem l ∘ req) (eq l ∘ ch))
+
+lemma scheduling
+  (sch : scheduler r)
+  (sem : system_sem (sch.s))
+: ∃ τ : stream lbl, fair (req_of r τ) τ :=
+@scheduling' lbl sch.s sch.sem _ sch.F sch.ch _ sch.PROG sch.INIT sch.STEP sch.INV
+
+end unity
 
 end scheduling
